coq/Corps/Types.v
@@ -1,8 +1,11 @@
 Require Import EqBool.
+Require Import Modalities.
 Require Import Syntax.
+Require Import Contexts.
 From Stdlib Require Import RelationClasses.
 From Stdlib Require Import Lia.
 From Stdlib Require Import Program.Equality.
+
 
 Section CorpsTypes.
   Context {PName : Type} `{EqBool PName}.
@@ -17,58 +20,69 @@ Section CorpsTypes.
   
   Section TypeSystem.
 
-    Inductive Typed : Ctxt -> expr -> type -> Prop :=
-    | VarTyping {Γ : Ctxt} {n : nat} {τ : type} (m : mod) (pf1 : vars Γ n = (m, τ)) (pf2 : locks Γ n = m)
-      : Typed Γ (var n) τ
-    | UnitTyping (Γ : Ctxt) : Typed Γ uu UnitT
-    | AtTyping {Γ : Ctxt} {e : expr} {τ : type} (p : PName) (pf : Typed (add_lock Γ p) e τ)
-      : Typed Γ (atE p e) (AtT p τ)
-    | LetTyping {Γ : Ctxt} {e1 e2 : expr} {τ σ : type} {p : PName}
-        (pf1 : Typed Γ e1 (AtT p τ)) (pf2 : Typed (add_var Γ p τ) e2 σ)
-      : Typed Γ (letAt p e1 e2) σ
-    | PairTyping {Γ : Ctxt} {e1 e2 : expr} {τ1 τ2 : type}
-        (pf1 : Typed Γ e1 τ1) (pf2 : Typed Γ e2 τ2)
-      : Typed Γ (pair e1 e2) (TimesT τ1 τ2)
-    | ProjLTyping {Γ : Ctxt} {e : expr} {τ1 τ2 : type}
-        (pf : Typed Γ e (TimesT τ1 τ2))
-      : Typed Γ (pi1 e) τ1
-    | ProjRTyping {Γ : Ctxt} {e : expr} {τ1 τ2 : type}
-        (pf : Typed Γ e (TimesT τ1 τ2))
-      : Typed Γ (pi2 e) τ2
-    | InlTyping {Γ : Ctxt} {e : expr} {τ1 τ2 : type}
-        (pf : Typed Γ e τ1)
-      : Typed Γ (inl e) (PlusT τ1 τ2)
-    | InrTyping {Γ : Ctxt} {e : expr} {τ1 τ2 : type}
-        (pf : Typed Γ e τ2)
-      : Typed Γ (inr e) (PlusT τ1 τ2)
-    | CaseTyping {Γ : Ctxt} {e1 e2 e3 : expr} {τ1 τ2 σ : type}
-        (pf1 : Typed Γ e1 (PlusT τ1 τ2))
-        (pf2 : Typed (add_var Γ base τ1) e2 σ)
-        (pf3 : Typed (add_var Γ base τ2) e3 σ)
-      : Typed Γ (caseE e1 e2 e3) σ
-    | EfqlTyping {Γ : Ctxt} {e : expr}
-        (pf : Typed Γ e VoidT) (τ : type)
-      : Typed Γ (efql e) τ
-    | LamTyping {Γ : Ctxt} {e : expr} {τ1 τ2 : type}
-        (pf : Typed (add_var Γ base τ1) e τ2)
-      : Typed Γ (lam τ1 e) (ArrT τ1 τ2)
-    | AppTyping {Γ : Ctxt} {e1 e2 : expr} {τ1 τ2 : type}
-        (pf1 : Typed Γ e1 (ArrT τ1 τ2))
-        (pf2 : Typed Γ e2 τ1)
-      : Typed Γ (appE e1 e2) τ2
-    | SendTyping {Γ : Ctxt} {p q : PName} {e : expr} {τ : type}
-        (pf : Typed Γ e (AtT p τ))
-        (cs : CanSend (cons (all_locks Γ) p) (cons (all_locks Γ) q))
-      : Typed Γ (send e p emptyFC q) (AtT q τ)
-    | UpTyping {Γ : Ctxt} {p : PName} {e : expr} {τ : type}
-        (cu : CanUp (all_locks Γ) (cons (all_locks Γ) p))
-        (pf : Typed Γ e τ)
-      : Typed Γ (up e p emptyFC) (AtT p τ)
-    | DownTyping {Γ : Ctxt} {p : PName} {e : expr} {τ : type}
-        (cd : CanDown (cons (all_locks Γ) p) (all_locks Γ))
-        (pf : Typed Γ e (AtT p τ))
-      : Typed Γ (down e p emptyFC) τ
+    Inductive TypedAtLevel : Ctxt -> nat -> expr -> type -> Prop :=
+    | VarTyping {Γ : Ctxt} {l n : nat} {τ : type} (m : mod) (pf1 : vars Γ n = (m, τ)) (pf2 : locks Γ n = m)
+      : TypedAtLevel Γ l (var n) τ
+    | UnitTyping (Γ : Ctxt) (l : nat) : TypedAtLevel Γ l uu UnitT
+    | AtTyping {Γ : Ctxt} {l : nat} {e : expr} {τ : type} (p : PName) (pf : TypedAtLevel (add_lock Γ p) l e τ)
+      : TypedAtLevel Γ l (atE p e) (AtT p τ)
+    | LetTyping {Γ : Ctxt} {l : nat} {e1 e2 : expr} {τ σ : type} {p : PName}
+        (pf1 : TypedAtLevel Γ l e1 (AtT p τ)) (pf2 : TypedAtLevel (add_var Γ p τ) (S l) e2 σ)
+      : TypedAtLevel Γ l (letAt p e1 e2) σ
+    | PairTyping {Γ : Ctxt} {l : nat} {e1 e2 : expr} {τ1 τ2 : type}
+        (pf1 : TypedAtLevel Γ l e1 τ1) (pf2 : TypedAtLevel Γ l e2 τ2)
+      : TypedAtLevel Γ l (pair e1 e2) (TimesT τ1 τ2)
+    | ProjLTyping {Γ : Ctxt} {l : nat} {e : expr} {τ1 τ2 : type}
+        (pf : TypedAtLevel Γ l e (TimesT τ1 τ2))
+      : TypedAtLevel Γ l (pi1 e) τ1
+    | ProjRTyping {Γ : Ctxt} {l : nat} {e : expr} {τ1 τ2 : type}
+        (pf : TypedAtLevel Γ l e (TimesT τ1 τ2))
+      : TypedAtLevel Γ l (pi2 e) τ2
+    | InlTyping {Γ : Ctxt} {l : nat} {e : expr} {τ1 τ2 : type}
+        (pf : TypedAtLevel Γ l e τ1)
+      : TypedAtLevel Γ l (inl e) (PlusT τ1 τ2)
+    | InrTyping {Γ : Ctxt} {l : nat} {e : expr} {τ1 τ2 : type}
+        (pf : TypedAtLevel Γ l e τ2)
+      : TypedAtLevel Γ l (inr e) (PlusT τ1 τ2)
+    | CaseTyping {Γ : Ctxt} {l : nat} {e1 e2 e3 : expr} {τ1 τ2 σ : type}
+        (pf1 : TypedAtLevel Γ l e1 (PlusT τ1 τ2))
+        (pf2 : TypedAtLevel (add_var Γ base τ1) (S l) e2 σ)
+        (pf3 : TypedAtLevel (add_var Γ base τ2) (S l) e3 σ)
+      : TypedAtLevel Γ l (caseE e1 e2 e3) σ
+    | EfqlTyping {Γ : Ctxt} {l : nat} {e : expr}
+        (pf : TypedAtLevel Γ l e VoidT) (τ : type)
+      : TypedAtLevel Γ l (efql e) τ
+    | LamTyping {Γ : Ctxt} {l : nat} {e : expr} {τ1 τ2 : type}
+        (pf : TypedAtLevel (add_var Γ base τ1) (S l) e τ2)
+      : TypedAtLevel Γ l (lam τ1 e) (ArrT τ1 τ2)
+    | AppTyping {Γ : Ctxt} {l : nat} {e1 e2 : expr} {τ1 τ2 : type}
+        (pf1 : TypedAtLevel Γ l e1 (ArrT τ1 τ2))
+        (pf2 : TypedAtLevel Γ l e2 τ1)
+      : TypedAtLevel Γ l (appE e1 e2) τ2
+    | SendTyping {Γ Γ' : Ctxt} {l seen : nat} {m : mod} {p q : PName}  {e : expr} {τ : type}
+        (locks_seen : locks Γ seen = cons m p)
+        (eqv : ctxt_equiv Γ' (change_lock Γ (change_lock_inv_send q locks_seen)))
+        (pf : TypedAtLevel Γ' l e τ)
+        (cs : CanSend (cons m p) (cons m q))
+        (seen_at_level : seen <= l)
+      : TypedAtLevel Γ l (send e seen m p q) τ
+    | UpTyping {Γ Γ' : Ctxt} {l seen : nat} {m : mod} {p : PName} {e : expr} {τ : type}
+        (locks_seen : locks Γ seen = m)
+        (eqv : ctxt_equiv Γ' (change_lock Γ (change_lock_inv_up p locks_seen)))
+        (pf : TypedAtLevel Γ' l e τ)
+        (cu : CanUp m (cons m p))
+        (seen_at_level : seen <= l)
+      : TypedAtLevel Γ l (up e seen m p) τ
+    | DownTyping {Γ Γ' : Ctxt} {l seen : nat} {m : mod} {p : PName} {e : expr} {τ : type}
+        (locks_seen : locks Γ seen = cons m p)
+        (eqv : ctxt_equiv Γ' (change_lock Γ (change_lock_inv_down locks_seen)))
+        (pf : TypedAtLevel Γ' l e τ)
+        (cu : CanDown (cons m p) m)
+        (seen_at_level : seen <= l)
+      : TypedAtLevel Γ l (down e seen m p) τ
     .
+
+    Definition Typed Γ e τ := TypedAtLevel Γ 0 e τ.
 
     Theorem add_lock_ext : forall (Γ Δ : Ctxt) m, ctxt_equiv Γ Δ -> ctxt_equiv (add_lock Γ m) (add_lock Δ m).
     Proof using.
@@ -86,17 +100,10 @@ Section CorpsTypes.
       all: auto.
     Qed.
 
-    Theorem add_finite_ctxt_ext : forall Γ Δ E,
-        ctxt_equiv Γ Δ -> ctxt_equiv (addFiniteCtxt Γ E) (@addFiniteCtxt PName Δ E).
+    Theorem type_level_ext : forall (Γ Δ : Ctxt) (l : nat) (e : expr) (τ : type),
+        TypedAtLevel Γ l e τ -> (ctxt_equiv Γ Δ) -> TypedAtLevel Δ l e τ.
     Proof using.
-      intros Γ Δ E; revert Γ Δ; induction E; intros Γ Δ eqv; cbn; auto;
-        apply IHE; [apply add_var_ext; auto | apply add_lock_ext; auto].
-    Qed.
-
-    Theorem type_ext : forall (Γ Δ : Ctxt) (e : expr) (τ : type),
-        Typed Γ e τ -> (ctxt_equiv Γ Δ) -> Typed Δ e τ.
-    Proof using.
-      intros Γ Δ e τ typd; revert Δ; induction typd; try (rename Δ into Γ'); intros Δ' eqv';
+      intros Γ Δ l e τ typd; revert Δ; induction typd; try (rename Δ into Γ'); intros Δ' eqv';
         pose proof (proj1 eqv') as vars_eq;
         pose proof (proj1 (proj2 eqv')) as locks_eq;
         pose proof (proj2 (proj2 eqv')) as all_locks_eq;
@@ -111,31 +118,37 @@ Section CorpsTypes.
               | [ _ : locks Δ n = x |- _ ] => fail
               | _ => assert (locks Δ n = x) by (rewrite <- H'; exact H)
               end
-          | [ IH : forall Δ, ctxt_equiv (add_lock ?Γ ?m) Δ -> Typed Δ ?e ?τ, H : ctxt_equiv ?Γ ?Δ |- _ ] =>
+          | [ IH : forall Δ, ctxt_equiv (add_lock ?Γ ?m) Δ -> TypedAtLevel Δ ?l ?e ?τ, H : ctxt_equiv ?Γ ?Δ |- _ ] =>
               lazymatch goal with
-              | [ _ : Typed (add_lock Δ m) e τ |- _ ] => fail
+              | [ _ : TypedAtLevel (add_lock Δ m) l e τ |- _ ] => fail
               | _ => pose proof (IH (add_lock Δ m) (add_lock_ext Γ Δ m H))
               end
-          | [ IH : forall Δ, ctxt_equiv (add_var ?Γ ?m ?τ') Δ -> Typed Δ ?e ?τ, H : ctxt_equiv ?Γ ?Δ |- _ ] =>
+          | [ IH : forall Δ, ctxt_equiv (add_var ?Γ ?m ?τ') Δ -> TypedAtLevel Δ ?level ?e ?τ, H : ctxt_equiv ?Γ ?Δ |- _ ] =>
               lazymatch goal with
-              | [ _ : Typed (add_var Δ m τ') e τ |- _ ] => fail
+              | [ _ : TypedAtLevel (add_var Δ m τ') level e τ |- _ ] => fail
               | _ => pose proof (IH (add_var Δ m τ') (add_var_ext Γ Δ m τ' H))
               end
-          | [ IH : forall Δ, ctxt_equiv (addFiniteCtxt ?Γ ?E) Δ -> Typed Δ ?e ?τ, H : ctxt_equiv ?Γ ?Δ |- _ ] =>
-              lazymatch goal with
-              | [ _ : Typed (addFiniteCtxt Δ E) e τ |- _ ] => fail
-              | _ => pose proof (IH (addFiniteCtxt Δ E) (add_finite_ctxt_ext Γ Δ E H))
-              end
+          (* | [ IH : forall Δ, ctxt_equiv (addFiniteCtxt ?Γ ?E) Δ -> TypedAtLevel Δ ?l ?e ?τ, H : ctxt_equiv ?Γ ?Δ |- _ ] => *)
+          (*     lazymatch goal with *)
+          (*     | [ _ : Typed (addFiniteCtxt Δ E) l e τ |- _ ] => fail *)
+          (*     | _ => pose proof (IH (addFiniteCtxt Δ E) (add_finite_ctxt_ext Γ Δ E H)) *)
+          (*     end *)
           end;
         try (econstructor; eauto; fail).
-      - apply @SendTyping with (Γ := Δ'); auto.
-        rewrite <- all_locks_eq; exact cs.
-      - apply @UpTyping with (Γ := Δ'); auto.
-        rewrite <- all_locks_eq; exact cu.
-      - apply @DownTyping with (Γ := Δ'); auto.
-        rewrite <- all_locks_eq; exact cd.
+      - apply @SendTyping with (Γ' := Γ') (locks_seen := H0); auto.
+        etransitivity; [exact eqv | apply change_lock_ext; auto].
+      - apply @UpTyping with (Γ' := Γ') (locks_seen := H0); auto.
+        etransitivity; [exact eqv | apply change_lock_ext; auto].
+      - apply @DownTyping with (Γ' := Γ') (locks_seen := H0); auto.
+        etransitivity; [exact eqv | apply change_lock_ext; auto].
     Qed.
 
+    Theorem type_ext : forall (Γ Δ : Ctxt) (e : expr) (τ : type),
+        Typed Γ e τ -> (ctxt_equiv Γ Δ) -> Typed Δ e τ.
+    Proof using.
+      intros Γ Δ e τ H0 H1; eapply type_level_ext; eauto.
+    Qed.
+    
     Definition ctxt_ren (Γ : Ctxt) (ξ : renaming) (mono : forall n m, n <= m -> PrefixOf (locks Γ (ξ n)) (locks Γ (ξ m))): Ctxt :=
       {|
         vars n := vars Γ (ξ n);
@@ -144,6 +157,12 @@ Section CorpsTypes.
         locks_mono n m lt := mono n m lt;
         locks_bound n := locks_bound Γ (ξ n);
       |}.
+
+    Lemma ctxt_ren_ext : forall Γ ξ mono mono',
+        ctxt_equiv (ctxt_ren Γ ξ mono) (ctxt_ren Γ ξ mono').
+    Proof using.
+      intros Γ ξ mono mono'; split; [| split]; cbn; reflexivity.
+    Qed.
 
     Lemma renup_mono : forall (ξ : renaming) (Γ : Ctxt) g τ, (forall n m, n <= m -> PrefixOf (locks Γ (ξ n)) (locks Γ (ξ m))) ->
                                                         forall n m, n <= m -> PrefixOf (locks (add_var Γ g τ) (renup ξ n)) (locks (add_var Γ g τ) (renup ξ m)).
@@ -163,52 +182,77 @@ Section CorpsTypes.
       cbn. apply PrefixOf_app_mono; auto.
     Qed.
 
-    Lemma weakening : forall (Γ Δ : Ctxt) (e : expr) (ξ : renaming) (τ : type) mono,
-        ctxt_equiv (ctxt_ren Γ ξ mono) Δ ->
-        Typed Δ e τ -> Typed Γ (ren e ξ) τ.
+    Lemma renup_nochange : forall ξ l, (forall n, n < l -> ξ n = n) -> forall n, n < S l -> renup ξ n = n.
     Proof using.
-      intros Γ Δ e ξ τ mono eqv typ; revert Γ ξ mono eqv; induction typ;
-        intros Γ'' ξ mono ctxt_eqv; cbn.
+      intros ξ l nochange n n_lt_Sl; destruct n; cbn; auto.
+      apply PeanoNat.lt_S_n in n_lt_Sl. rewrite nochange. reflexivity. exact n_lt_Sl.
+    Qed.
+
+    Lemma nolocks_change_mono : forall {Γ : Ctxt} {ξ : renaming},
+        (forall n, locks Γ n = locks Γ (ξ n)) ->
+        forall n m, n <= m -> PrefixOf (locks Γ (ξ n)) (locks Γ (ξ m)).
+    Proof using.
+      intros Γ ξ H0 n m H1; repeat rewrite <- H0; apply locks_mono; exact H1.
+    Qed.
+
+
+    Lemma weakening_at_level : forall (Γ Δ : Ctxt) (l : nat) (e : expr) (ξ : renaming) (τ : type)
+                                 (locks_no_change : forall n, locks Γ n = locks Γ (ξ n)),
+        ctxt_equiv (ctxt_ren Γ ξ (nolocks_change_mono locks_no_change)) Δ ->
+        (forall n, n < l -> ξ n = n) ->
+        TypedAtLevel Δ l e τ -> TypedAtLevel Γ l (ren e ξ) τ.
+    Proof using.
+      intros Γ Δ l e ξ τ mono eqv ξ_eq typ; revert Γ ξ mono eqv ξ_eq; induction typ; try rename Γ'' into Γ2;
+        intros Γ'' ξ mono ctxt_eqv ξ_eq; cbn.
       all: pose proof ctxt_eqv as [vars_eqv [locks_eqv al_eqv]].
       all: try (econstructor; eauto; fail).
-      - apply VarTyping with (m := m).  rewrite <- pf1; rewrite <- vars_eqv; cbn; reflexivity.
-        rewrite <- pf2; rewrite <- locks_eqv; cbn; reflexivity.
-      - apply AtTyping. eapply IHtyp. Unshelve.
-        2: { intros n m H0; cbn; apply mod_app_mono_l; apply mono; auto. }
-        split; [|split].
-        -- intro x; cbn. rewrite <- vars_eqv. cbn. reflexivity.
-        -- intro x; cbn. rewrite <- locks_eqv. cbn. reflexivity.
-        -- unfold ctxt_ren; cbn. f_equal.
-           rewrite <- al_eqv. unfold ctxt_ren; cbn; reflexivity.
       - econstructor; eauto.
-        apply IHtyp2 with (mono := renup_mono ξ Γ'' p τ mono).
-        split; [|split]; auto.
-        all: intro x; destruct x; cbn; auto.
-        -- rewrite <- vars_eqv; unfold ctxt_ren; cbn; auto.
-        -- rewrite <- locks_eqv; unfold ctxt_ren; cbn; auto.
-      - eapply CaseTyping;
-          [
-            eapply IHtyp1; eauto
-          | apply IHtyp2 with (mono := renup_mono ξ Γ'' base τ1 mono)
-          | eapply IHtyp3 with (mono := renup_mono ξ Γ'' base τ2 mono)
-          ].
-        all: split; [|split]; auto; intro x; destruct x; cbn; auto.
-        1, 3: apply vars_eqv; auto.
-        all: apply locks_eqv; auto.
-      - eapply LamTyping.
-        apply IHtyp with (mono := renup_mono ξ Γ'' base τ1 mono).
-        split; [|split]; auto.
-        -- intro x; destruct x; cbn; auto.
-           cbn in vars_eqv; apply vars_eqv.
-        -- intro x; destruct x; cbn; auto.
-           apply locks_eqv.
-      - cbn in *; eapply @SendTyping with (Γ := Γ''); eauto.
-        rewrite al_eqv; auto.
-      - cbn in *; eapply @UpTyping with (Γ := Γ''); eauto.
-        rewrite al_eqv; auto.
-      - cbn in *; eapply @DownTyping with (Γ := Γ''); eauto.
-        rewrite al_eqv; auto.
-    Qed.
+        rewrite <- mono.
+        specialize (vars_eqv n); cbn in vars_eqv; rewrite vars_eqv.
+        specialize (locks_eqv n); cbn in locks_eqv; rewrite locks_eqv.
+        rewrite pf1. rewrite pf2. reflexivity.
+      - econstructor; eauto.
+        eapply IHtyp; eauto.
+        split; [| split]; cbn; eauto.
+        2: cbn in al_eqv; rewrite al_eqv; reflexivity.
+        intro x; specialize (locks_eqv x); cbn in locks_eqv; rewrite locks_eqv; reflexivity.
+        Unshelve. cbn; intro n; rewrite <- mono; reflexivity.
+      - econstructor; eauto.
+        eapply IHtyp2. 2: apply renup_nochange; auto. split; [| split]; try intro x; cbn; auto.
+        all: destruct x; cbn; auto. apply vars_eqv. apply locks_eqv.
+        Unshelve. intro n; cbn; destruct n; cbn; [reflexivity | apply mono].
+      - econstructor; eauto.
+        eapply IHtyp2. 3: eapply IHtyp3. all: try eapply renup_nochange; eauto.
+        all: split; [| split]; try intro x; cbn; try reflexivity; try destruct x; cbn; auto.
+        1,3: apply vars_eqv. all: apply locks_eqv.
+        Unshelve. all: intro n; destruct n; cbn; auto.
+      - econstructor; eauto.
+        eapply IHtyp; [|apply renup_nochange; auto].
+        split; [| split]; try intro x; cbn; auto; destruct x; cbn; auto.
+        apply vars_eqv. apply locks_eqv.
+        Unshelve. intro n; destruct n; cbn; auto.
+      - assert (locks Γ'' (ξ seen) = cons m p) as locks_seen'
+            by (specialize (locks_eqv seen); cbn in locks_eqv;
+                rewrite locks_eqv; apply locks_seen).
+        assert (locks Γ'' seen = cons m p) as locks_seen''
+            by (rewrite mono; apply locks_seen').
+        eapply @SendTyping with (Γ' := change_lock Γ'' (change_lock_inv_send q locks_seen'')); eauto;
+          [reflexivity|].
+        eapply IHtyp; auto.
+        destruct eqv as [vars_eqv' [locks_eqv' al_eqv']].
+        split; [| split]; cbn; try intro x.
+        -- specialize (vars_eqv x); cbn in vars_eqv; rewrite vars_eqv.
+           specialize (vars_eqv' x); cbn in vars_eqv'; symmetry; apply vars_eqv'.
+        -- specialize (locks_eqv x); cbn in locks_eqv; rewrite locks_eqv.
+           specialize (locks_eqv' x); cbn in locks_eqv'.
+           symmetry; apply locks_eqv'.
+        -- cbn in al_eqv; rewrite al_eqv; cbn in al_eqv'; symmetry; apply al_eqv'.
+           Unshelve. intro n; cbn; rewrite <- mono; reflexivity.
+      - 
+          
+        
+        
+        
 
   End TypeSystem.
 
