coq/Corps/Contexts.v
@@ -1,0 +1,270 @@
+Require Import Base.EqBool.
+From Stdlib Require Import Lists.List.
+From Stdlib Require Import Lia.
+From Stdlib Require Import Classes.RelationClasses.
+Import ListNotations.
+From Stdlib Require Import Logic.JMeq.
+From Stdlib Require Import Logic.Eqdep_dec.
+From Stdlib Require Import Program.Equality.
+From Stdlib Require Import Program.Wf.
+
+Require Import Modalities.
+Require Import Syntax.
+
+Section Contexts.
+  Context {PName : Type} `{EqBool PName}.
+  #[local] Notation mod := (@mod PName).
+  #[local] Definition ptm := @proc_to_mod PName.
+  #[local] Definition PrefixOfT := @PrefixOfT PName.
+  Coercion ptm : PName >-> mod.
+  #[local] Notation type := (type PName).
+  #[local] Notation expr := (expr PName).
+
+  Record Ctxt :=
+    {
+      vars : nat -> mod * type;
+      locks : nat -> mod;
+      all_locks : mod;
+      locks_mono : forall {n m}, n <= m -> PrefixOf (locks n) (locks m);
+      locks_bound : forall n, PrefixOf (locks n) all_locks
+    }.
+  
+  Definition add_lock (Γ : Ctxt) (m : mod) : Ctxt :=
+    {|
+      vars n := vars Γ n;
+      locks n := mod_app m (locks Γ n);
+      all_locks := mod_app m (all_locks Γ);
+      locks_mono := fun j k leq => PrefixOf_app_mono m (locks_mono Γ leq);
+      locks_bound := fun n => PrefixOf_app_mono m (locks_bound Γ n); 
+    |}.
+  
+  Definition remove_lock (Γ : Ctxt) (m : mod) : option Ctxt.
+    refine (match PrefixOfT_dec m (locks Γ 0) with
+            | None => None
+            | Some pfx =>
+                Some ({|
+                      vars n :=  vars Γ n;
+                      locks n := @remove_PrefixT PName m (locks Γ n) (prefixT_prefix_trans pfx (@locks_mono Γ 0 n ltac:(lia)));
+                      all_locks := @remove_PrefixT PName m (all_locks Γ) (prefixT_prefix_trans pfx (@locks_bound Γ 0));
+                      locks_mono := _;
+                      locks_bound := _;
+                    |})
+            end).
+    - intros n m0 H0; apply remove_prefix_mono; apply (locks_mono Γ H0).
+    - intros n; apply remove_prefix_mono; apply (locks_bound Γ).
+  Defined.
+
+  Program Definition add_var (Γ : Ctxt) (m : mod) (τ : type) : Ctxt :=
+    {|
+      vars n :=
+        match n with
+        | 0 => (m, τ)
+        | S n' => vars Γ n'
+        end;
+      locks n :=
+        match n with
+        | 0 => base
+        | S n' => locks Γ n'
+        end;
+      all_locks := all_locks Γ;
+    |}.
+  Next Obligation.
+    induction H0. destruct n; reflexivity.
+    destruct n. apply base_Prefix.
+    apply locks_mono; lia.
+  Defined.
+  Next Obligation.
+    destruct n; [apply base_Prefix | apply locks_bound].
+  Qed.
+
+  Definition ctxt_equiv (Γ Δ : Ctxt) : Prop :=
+    (forall x, vars Γ x = vars Δ x)
+    /\ (forall x, locks Γ x = locks Δ x)
+    /\ all_locks Γ = all_locks Δ.
+
+  Lemma ctxt_equiv_refl (Γ : Ctxt) : ctxt_equiv Γ Γ.
+  Proof using.
+    split; [|split]; intros; reflexivity.
+  Qed.
+
+  #[global] Instance CtxtEquivRefl : Reflexive ctxt_equiv := ctxt_equiv_refl.
+
+  Lemma ctxt_equiv_symm : forall Γ Δ : Ctxt, ctxt_equiv Γ Δ -> ctxt_equiv Δ Γ.
+  Proof using.
+    intros Γ Δ [vars_eqv [locks_eqv all_locks_eqv]];
+      split; [| split]; intros; symmetry; auto.
+  Qed.
+
+  #[global] Instance CtxtEquivSym : Symmetric ctxt_equiv := ctxt_equiv_symm.
+
+  Lemma ctxt_equiv_trans : forall Γ Δ E : Ctxt, ctxt_equiv Γ Δ -> ctxt_equiv Δ E -> ctxt_equiv Γ E.
+  Proof using.
+    intros Γ Δ E [vars_eqv1 [locks_eqv1 all_locks_eqv1]] [vars_eqv2 [locks_eqv2 all_locks_eqv2]];
+      split; [|split]; intros; etransitivity; eauto.
+  Qed.
+
+  #[global] Instance CtxtEquivTrans : Transitive ctxt_equiv := ctxt_equiv_trans.
+
+  #[global] Instance CtxtEquivEquiv : Equivalence ctxt_equiv :=
+    {|
+      Equivalence_Reflexive := CtxtEquivRefl;
+      Equivalence_Symmetric := CtxtEquivSym;
+      Equivalence_Transitive := CtxtEquivTrans;
+    |}.
+
+  Lemma add_base_lock : forall Γ, ctxt_equiv Γ (add_lock Γ base).
+  Proof using.
+    intro Γ; split; [|split]; intros; cbn; try rewrite mod_base_app; reflexivity.
+  Qed.
+
+  Lemma add_two_locks : forall Γ m1 m2, ctxt_equiv (add_lock Γ (mod_app m1 m2)) (add_lock (add_lock Γ m2) m1).
+  Proof using.
+    intros Γ m1 m2; split; [|split]; intros; cbn; try reflexivity; apply mod_app_assoc.
+  Qed.
+
+
+  
+  Section Lockpointer.
+
+    Record lockpointer (Γ : Ctxt) (m : mod) :=
+      {
+        index : nat;
+        prefix : mod;
+        pred_index : (index = 0 /\ prefix = base) \/ (exists k, index = S k /\ locks Γ k = prefix);
+        at_index : locks Γ index = mod_app prefix m
+      }.
+
+    Lemma before_index : forall (Γ : Ctxt) (m : mod) (ptr : lockpointer Γ m) (n : nat),
+        n < index Γ m ptr ->
+        PrefixOf (locks Γ n) (prefix Γ m ptr).
+    Proof using.
+      intros Γ m ptr n n_lt_index.
+      destruct (pred_index Γ m ptr) as [[eq0 eq_base] | [k [eqS eq_locks]]].
+      - rewrite eq0 in n_lt_index; inversion n_lt_index.
+      - transitivity (locks Γ k).
+        -- apply locks_mono; rewrite eqS in n_lt_index; apply PeanoNat.lt_n_Sm_le; exact n_lt_index.
+        -- rewrite eq_locks; reflexivity.
+    Qed.
+
+    
+    Program Definition change_lock (Γ : Ctxt) {m1 m2 : mod} (inv : forall n, PrefixOf m1 (locks Γ n) \/ PrefixOf (locks Γ n) m2) :=
+      {|
+        vars := vars Γ;
+        locks n :=
+          match change_prefix m1 (locks Γ n) m2 with
+          | Some m => m
+          | None => locks Γ n
+          end;
+        all_locks := match change_prefix m1 (all_locks Γ) m2 with
+                    | Some m => m
+                    | None => all_locks Γ
+                    end
+      |}.
+    Next Obligation.
+      destruct (change_prefix m1 (locks Γ n) m2) eqn:eq0;
+        destruct (change_prefix m1 (locks Γ m) m2) eqn:eq1.
+      - apply change_prefix_of_prefix' with (m1 := m1) (m3 := m2) (m2 := locks Γ n) (m2' := locks Γ m);
+          auto; apply locks_mono; auto.
+      - apply only_prefixes_changable in eq0.
+        assert (PrefixOf m1 (locks Γ m)) 
+          by (transitivity (locks Γ n); [exact eq0 | apply locks_mono; exact H0]).
+        exfalso; apply change_prefix_of_prefix in eq1; auto.
+      - destruct (inv n);
+          [exfalso; apply change_prefix_of_prefix in eq0; auto|].
+        apply prefix_changed_to_prefix in eq1.
+        transitivity m2; auto.
+      - apply locks_mono; exact H0.
+    Qed.
+    Next Obligation.
+      destruct (change_prefix m1 (locks Γ n) m2) eqn:eq0;
+        destruct (change_prefix m1 (all_locks Γ) m2) eqn:eq1.
+      - apply change_prefix_of_prefix' with (m1 := m1) (m2 := locks Γ n) (m2' := all_locks Γ) (m3 := m2);
+          auto; apply locks_bound.
+      - exfalso. apply only_prefixes_changable in eq0.
+        apply change_prefix_of_prefix in eq1; auto.
+        transitivity (locks Γ n); auto. apply locks_bound.
+      - destruct (inv n); [exfalso; apply change_prefix_of_prefix in eq0; auto|].
+        apply prefix_changed_to_prefix in eq1; transitivity m2; auto.
+      - apply locks_bound.
+    Qed.
+
+    Lemma inv_ext : forall  {Γ Δ : Ctxt} {m1 m2 : mod},
+        ctxt_equiv Γ Δ ->
+        (forall n, PrefixOf m1 (locks Γ n) \/ PrefixOf (locks Γ n) m2) ->
+        forall n, PrefixOf m1 (locks Δ n) \/ PrefixOf (locks Δ n) m2.
+    Proof using.
+      intros Γ Δ m1 m2 [vars_equiv [locks_equiv al_eqv]] Γ_inv n.
+      destruct (Γ_inv n) as [pfx | pfx]; [left | right]; rewrite <- locks_equiv; auto.
+    Qed.
+    
+    Lemma change_lock_inv_ext : forall {Γ : Ctxt} {m1 m2 : mod} (inv1 inv2 : forall n, PrefixOf m1 (locks Γ n) \/ PrefixOf (locks Γ n) m2),
+        ctxt_equiv (change_lock Γ inv1) (change_lock Γ inv2).
+    Proof using.
+      intros Γ m1 m2 inv1 inv2; destruct Γ; cbn in *.
+      split; [| split]; try intro x; cbn; auto.
+    Qed.
+
+    Lemma change_lock_ctxt_ext : forall {Γ Δ : Ctxt} {m1 m2 : mod} (inv : forall n, PrefixOf m1 (locks Γ n) \/ PrefixOf (locks Γ n) m2)
+                                        (eqv : ctxt_equiv Γ Δ),
+        ctxt_equiv (change_lock Γ inv) (change_lock Δ (inv_ext eqv inv)).
+    Proof using.
+      intros Γ Δ m1 m2 inv [vars_eqv [locks_eqv al_eqv]].
+      split; [| split]; try intro x; cbn; auto.
+      rewrite locks_eqv; reflexivity.
+      rewrite al_eqv; reflexivity.
+    Qed.
+
+    Lemma change_lock_ext : forall {Γ Δ : Ctxt} {m1 m2 : mod} (inv1 : forall n, PrefixOf m1 (locks Γ n) \/ PrefixOf (locks Γ n) m2)
+                              (inv2 : forall n, PrefixOf m1 (locks Δ n) \/ PrefixOf (locks Δ n) m2),
+        ctxt_equiv Γ Δ ->
+        ctxt_equiv (change_lock Γ inv1) (change_lock Δ inv2).
+    Proof using.
+      intros Γ Δ m1 m2 inv1 inv2 eqv;
+        transitivity (change_lock Δ (inv_ext eqv inv1)); [apply change_lock_ctxt_ext | apply change_lock_inv_ext].
+    Qed.
+    
+    Theorem change_lock_inv_send : forall {Γ : Ctxt} {m : mod} {p : PName} (q : PName) {seen : nat},
+        locks Γ seen = cons m p ->
+        forall n, PrefixOf (cons m p) (locks Γ n)  \/ PrefixOf (locks Γ n) (cons m q).
+    Proof using.
+      intros Γ m p q seen seen_cons n.
+      destruct (PeanoNat.Nat.leb_spec n seen).
+      pose proof (locks_mono Γ H0) as prefix_n_seen; dependent destruction prefix_n_seen.
+      - left; rewrite x; rewrite seen_cons; reflexivity.
+      - rewrite seen_cons in x; inversion x; subst; clear x.
+        right. apply PO_step. exact prefix_n_seen.
+      - left; transitivity (locks Γ seen). rewrite seen_cons; reflexivity.
+        apply locks_mono; apply PeanoNat.Nat.lt_le_incl; exact H0.
+    Qed.           
+
+    Theorem change_lock_inv_up : forall {Γ : Ctxt} {m : mod} (p : PName) {seen : nat},
+        locks Γ seen = m ->
+        forall n, PrefixOf m (locks Γ n) \/ PrefixOf (locks Γ n) (cons m p).
+    Proof using.
+      intros Γ m p seen seen_cons n.
+      destruct (PeanoNat.Nat.leb_spec n seen) as [n_le_seen | seen_lt_n].
+      - pose proof (locks_mono Γ n_le_seen) as prefix_n_seen; dependent destruction prefix_n_seen.
+        -- left; rewrite <- seen_cons; rewrite <- x; reflexivity.
+        -- rewrite seen_cons in x; inversion x; subst.
+           right; do 2 apply PO_step; exact prefix_n_seen.
+      - left; transitivity (locks Γ seen). rewrite seen_cons; reflexivity.
+        apply locks_mono; apply PeanoNat.Nat.lt_le_incl; exact seen_lt_n.
+    Qed.
+
+    Theorem change_lock_inv_down : forall {Γ : Ctxt} {m : mod} {p : PName} {seen : nat},
+        locks Γ seen = cons m p ->
+        forall n, PrefixOf (cons m p) (locks Γ n) \/ PrefixOf (locks Γ n) m.
+    Proof using.
+      intros Γ m p seen locks_seen n.
+      destruct (PeanoNat.Nat.leb_spec n seen) as [n_le_seen | seen_lt_n].
+      - pose proof (locks_mono Γ n_le_seen) as prefix_n_seen; dependent destruction prefix_n_seen.
+        -- left; rewrite <- locks_seen; rewrite <- x; reflexivity.
+        -- rewrite locks_seen in x; inversion x; subst; clear x.
+           right; auto.
+      - left; transitivity (locks Γ seen). rewrite locks_seen; reflexivity.
+        apply locks_mono; apply PeanoNat.Nat.lt_le_incl; exact seen_lt_n.
+    Qed.    
+
+  End Lockpointer.
+
+End Contexts.
